Disjoint_union_right is now proven automatically with disjoint_union_left

Lampe/Lampe/SeparationLogic/LawfulHeap.lean
@@ -11,8 +11,7 @@ class LawfulHeap (α : Type _) where
   union_assoc {s₁ s₂ s₃ : α} : union (union s₁ s₂) s₃ = union s₁ (union s₂ s₃)
   disjoint_symm_iff {a b : α} : disjoint a b ↔ disjoint b a
   union_comm_of_disjoint {s₁ s₂ : α} : disjoint s₁ s₂ → union s₁ s₂ = union s₂ s₁
-  disjoint_union_left (x y z : α) : disjoint (union x y) z ↔ disjoint x z ∧ disjoint y z -- one of them should be enough
-  disjoint_union_right (x y z : α) : disjoint x (union y z) ↔ disjoint x y ∧ disjoint x z
+  disjoint_union_left (x y z : α) : disjoint (union x y) z ↔ disjoint x z ∧ disjoint y z
   disjoint_empty (x : α) : disjoint empty x
 
 instance [LawfulHeap α] : Union α := ⟨LawfulHeap.union⟩
@@ -52,7 +51,14 @@ theorem LawfulHeap_disjoint_union_left [LawfulHeap α] (x y z : α) :
 
 theorem LawfulHeap_disjoint_union_right [LawfulHeap α] (x y z : α) :
   LawfulHeap.disjoint x (y ∪ z) ↔ LawfulHeap.disjoint x y ∧ LawfulHeap.disjoint x z := by
-  simp [Union.union]
-  apply LawfulHeap.disjoint_union_right
+  conv =>
+    lhs
+    rw [LawfulHeap.disjoint_symm_iff]
+  conv =>
+    rhs
+    rw [LawfulHeap.disjoint_symm_iff]
+    rhs
+    rw [LawfulHeap.disjoint_symm_iff]
+  apply LawfulHeap.disjoint_union_left
 
 end Lampe
